thy/Bitmagic/WordInterval_NumberWang.thy
@@ -1,6 +1,6 @@
 theory WordInterval_NumberWang
 imports WordInterval
-  "./l4v/lib/WordLemmaBucket"
+  "./l4v/lib/Word_Lib/Word_Lemmas"
   WordInterval_Lists
 begin
 
@@ -20,12 +20,12 @@ context begin
      apply(simp)
      apply(subst(asm) Word.word_less_nat_alt)
      apply simp
-    apply(subst WordLemmaBucket.upto_enum_set_conv2[symmetric])
+    apply(subst Word_Lemmas.upto_enum_set_conv2[symmetric])
     apply(subst List.card_set)
     apply(simp add: remdups_enum_upto)
     done
 
-  lemma finite_wordinterval: "finite (wordinterval_to_set r)" using WordLemmaBucket.finite_word by simp
+  lemma finite_wordinterval: "finite (wordinterval_to_set r)" by simp
 
   fun wordinterval_card :: "('a::len) wordinterval \<Rightarrow> nat" where
     "wordinterval_card (WordInterval s e) = Suc (unat e) - (unat s)" |
